save

Array_Safe.thy
@@ -4,8 +4,11 @@ begin
 
 (* TODO: Use locale? *)
 
-definition array_nth_safe where
-  "array_nth_safe arr i = do {
+context
+begin
+
+qualified definition lookup where
+  "lookup arr i = do {
     len \<leftarrow> Array.len arr;
     if i < len
     then Array.nth arr i
@@ -15,8 +18,8 @@ definition array_nth_safe where
     }
   }"
 
-definition array_update_safe where
-  "array_update_safe i v arr = do {
+qualified definition update where
+  "update i v arr = do {
     len \<leftarrow> Array.len arr;
     if i < len
     then Array.upd i v arr
@@ -28,16 +31,18 @@ lemma nth_undefined: "i \<ge> length xs \<Longrightarrow> xs ! i = undefined(i -
   apply(induction xs arbitrary: i)
   by(auto split: nat.split)
 
-lemma array_nth_safe [sep_heap_rules]: "
+lemma lookup [sep_heap_rules]: "
    <arr \<mapsto>\<^sub>a xs> 
-    array_nth_safe arr i
+    lookup arr i
    <\<lambda>res. \<up>(res = xs ! i) * arr \<mapsto>\<^sub>a xs>"
-  unfolding array_nth_safe_def
+  unfolding lookup_def
   by sep_auto
 
 lemma array_update_safe [sep_heap_rules]:
-  "<arr \<mapsto>\<^sub>a xs> array_update_safe i v arr <\<lambda>res. \<up>(res = arr) * arr \<mapsto>\<^sub>a xs[i := v]>"
-  unfolding array_update_safe_def
+  "<arr \<mapsto>\<^sub>a xs> update i v arr <\<lambda>res. \<up>(res = arr) * arr \<mapsto>\<^sub>a xs[i := v]>"
+  unfolding update_def
   by sep_auto
+
+end
 
 end
