Example_CYK.thy
@@ -22,6 +22,77 @@ fun member' :: "'a \<Rightarrow> 'a list \<Rightarrow> bool" where
     | x#xs \<Rightarrow> (x = a \<or> member' a xs)
   )" 
 
+fun member'' :: "'a \<Rightarrow> 'a list \<Rightarrow> nat \<Rightarrow> bool" where
+  "member'' a xs n = (case n of 
+            0 \<Rightarrow> False 
+         | (Suc n) \<Rightarrow> (xs ! n = a \<or> member'' a xs n)
+  )"
+print_theorems
+declare member''.simps[simp del]
+
+
+definition member''_body where
+  "member''_body r a xs n =  (
+    case n of
+      0 \<Rightarrow> False
+    | (Suc n) \<Rightarrow> (let c1 = xs ! n; c2 = (c1 = a); c3 = r n; c4 = c2 \<or> c3 in c4)
+  )"
+
+definition member'_body where
+  "member'_body r a xs =  (
+    case xs of
+      [] \<Rightarrow> False
+    | x#xs \<Rightarrow> (x = a \<or> r a xs)
+  )"
+
+lemma member'_body: "member' = member'_body member'"
+  unfolding member'_body_def fun_eq_iff
+  by auto
+
+lemma member''_body: "member'' a xs = member''_body (member'' a xs) a xs"
+  unfolding member''_body_def fun_eq_iff Let_def
+  by(auto simp: member''.simps)
+
+lemma member'_induct:
+  assumes "\<And>xs r. (\<And>xs'. length xs' < length xs \<Longrightarrow> P (r a xs')) \<Longrightarrow> P (member'_body r a xs)"
+  shows "P (member' a xs)"
+  apply(induction "length xs" arbitrary: xs rule: nat_less_induct)
+  apply(subst member'_body)
+  apply(rule assms)
+  by auto
+
+lemma member_refinement:
+  assumes 
+    mono: "\<And>xs. mono_Heap (\<lambda>f. member'_bodyi f xs)"
+  and
+    step: "\<And>r ri xs xsi. (\<And>xs' xsi'. length xs' < length xs \<Longrightarrow> hnr (\<Gamma> xs' xsi') (ri xsi')  (\<Gamma>' xs' xsi') (r a xs')) 
+    \<Longrightarrow> hnr (\<Gamma> xs xsi) (member'_bodyi ri xsi) (\<Gamma>' xs xsi) (member'_body r a xs)"
+  shows "hnr (\<Gamma> xs xsi) (heap.fixp_fun member'_bodyi xsi) (\<Gamma>' xs xsi) (member' a xs)"
+  apply(induction "length xs" arbitrary: xs xsi rule: nat_less_induct)
+  apply(rewrite heap.mono_body_fixp[OF mono])
+  apply(rewrite member'_body)
+  apply(rule step)
+  by simp
+  
+lemma member''_refinement:
+  assumes 
+    mono: "\<And>xs. mono_Heap (\<lambda>f. member''_bodyi f xs)"
+  and
+    step: "\<And>r ri n. (\<And>n'. n' < n \<Longrightarrow> hnr (\<Gamma>) (ri n')  (\<Gamma>') (r n')) 
+    \<Longrightarrow> hnr (\<Gamma>) (member''_bodyi ri n) (\<Gamma>') (member''_body r a xs n)"
+  shows "hnr (\<Gamma>) (heap.fixp_fun member''_bodyi n) (\<Gamma>') (member'' a xs n)"
+  apply(induction n rule: nat_less_induct)
+  apply(rewrite heap.mono_body_fixp[OF mono])
+  apply(rewrite member''_body)
+  apply(rule step)
+  by simp
+
+lemma 
+    "hnr (master_assn' (insert (xs, xsi) F)) (c  xsi) \<Gamma>' (member' x xs)"
+  
+  apply(induction rule: member'_induct)
+  sorry
+
 fun match_prods :: "('n, 't) CNG \<Rightarrow> 'n list \<Rightarrow> 'n list \<Rightarrow> 'n list" where 
   "match_prods [] ls rs = []" 
 | "match_prods ((X, NonTerminals A B)#ps) ls rs = (
@@ -41,8 +112,20 @@ by pat_completeness auto
 termination 
 by(relation "measure(\<lambda>(a, b, c, d, e). e - d)", rule wf_measure, simp)
 
+context
+  fixes x :: "'a :: heap"
+begin
+
+
 synth_definition member'_impl is [hnr_rule_diff_arr]: 
-    "hnr (master_assn' (insert (xs, xsi) F)) (\<hole> :: ?'a Heap) ?\<Gamma>' (member' x xs)"
+    "hnr (master_assn' (insert (xs, xsi) F)) ((\<hole>  xsi):: ?'a Heap) ?\<Gamma>' (member'' x xs n)"
+  apply(rule member''_refinement)
+   defer
+  unfolding member''_body_def
+   apply hnr_diff_arr
+  apply(subgoal_tac "c1 = xi", hypsubst)
+          apply(rule hnr_return)
+         defer
   apply hnr_diff_arr
   done
 
