Test_Hnr.thy
@@ -116,6 +116,9 @@ definition create_arr where
 definition create_arr_2 where
   "create_arr_2 x = New_Arr [x]"
 
+definition create_arr_3 :: "('a::heap) \<Rightarrow> ('b::heap) \<Rightarrow> 'a list * 'b list" where
+  "create_arr_3 a b = (let xs = New_Arr [a]; ys = New_Arr [b] in (xs, ys))"
+
 definition create_diff_arr_empty :: "('a::heap) list" where
   "create_diff_arr_empty = New_Diff_Arr []" 
 
@@ -127,6 +130,9 @@ definition create_diff_arr_2 ::  "'a::heap \<Rightarrow> 'a list list" where
 
 definition create_diff_arr_3 :: "('a::heap) list" where
   "create_diff_arr_3 = (let xs = New_Diff_Arr [] in xs)"
+
+definition create_diff_arr_4 :: "('a::heap) \<Rightarrow> ('b::heap) \<Rightarrow> 'a list * 'b list" where
+  "create_diff_arr_4 a b = (let xs = New_Diff_Arr [a]; ys  = New_Diff_Arr [b] in (xs, ys))"
 
 definition create_arr_diff_arr :: "('a::heap) \<Rightarrow> 'a list" where
   "create_arr_diff_arr xs = (let a = New_Arr [xs]; b = Diff_Arr_From_Arr a in b)" 
@@ -207,7 +213,7 @@ synth_definition if_6_arr is
   unfolding if_6_def 
   by hnr_arr
 
-(* TODO: There is something wrong here \<Longrightarrow> I should reconsider the return-fallback  *)
+(* Shouldn't work, not linear! *)
 synth_definition if_7_arr is
   "hnr (array_assn xs xsi) (\<hole> :: ?'a Heap) ?\<Gamma>' (if_7 xs)"
   unfolding if_7_def 
@@ -238,6 +244,12 @@ synth_definition create_arr_2_impl is [hnr_rule_arr]:
   unfolding create_arr_2_def 
   by hnr_arr
 
+(* TODO: This somehow just works with diff arrays *)
+synth_definition create_arr_3_impl is [hnr_rule_arr]:
+  "hnr emp (\<hole> :: ?'a Heap) ?\<Gamma>' (create_arr_3 (x :: 'a :: heap))"
+  unfolding create_arr_3_def 
+  by hnr_arr
+
 (* HNR Diff-Array *)
 
 synth_definition sequential_1_diff_arr is [hnr_rule_diff_arr]:
@@ -246,52 +258,52 @@ synth_definition sequential_1_diff_arr is [hnr_rule_diff_arr]:
   by hnr_diff_arr
 
 synth_definition sequential_2_diff_arr is [hnr_rule_diff_arr]: 
-  "hnr (master_assn' {(xs, xsi)}) (\<hole> :: ?'a Heap) ?\<Gamma>' (sequential_2 xs)"
+  "hnr (master_assn' (insert (xs, xsi) F)) (\<hole> :: ?'a Heap) ?\<Gamma>' (sequential_2 xs)"
   unfolding sequential_2_def
   by hnr_diff_arr
 
 synth_definition return_tuple_1_diff_arr is [hnr_rule_diff_arr]: 
-  "hnr(master_assn' {(xs, xsi)}) (\<hole> :: ?'a Heap) ?\<Gamma>' (return_tuple_1 xs)"
+  "hnr (master_assn' (insert (xs, xsi) F)) (\<hole> :: ?'a Heap) ?\<Gamma>' (return_tuple_1 xs)"
   unfolding return_tuple_1_def
   by hnr_diff_arr
 
 synth_definition return_tuple_2_diff_arr is [hnr_rule_diff_arr]:
-  "hnr (master_assn' {(xs, xsi)}) (\<hole> :: ?'a Heap) ?\<Gamma>' (return_tuple_2 xs)"
+  "hnr (master_assn' (insert (xs, xsi) F)) (\<hole> :: ?'a Heap) ?\<Gamma>' (return_tuple_2 xs)"
   unfolding return_tuple_2_def 
   by hnr_diff_arr
    
 synth_definition return_tuple_3_diff_arr is [hnr_rule_diff_arr]: 
-  "hnr (master_assn' {(xs, xsi)}) (\<hole> :: ?'a Heap) ?\<Gamma>' (return_tuple_3 xs)"
+  "hnr (master_assn' (insert (xs, xsi) F)) (\<hole> :: ?'a Heap) ?\<Gamma>' (return_tuple_3 xs)"
   unfolding return_tuple_3_def 
   by hnr_diff_arr
 
 synth_definition return_tuple_4_diff_arr is [hnr_rule_diff_arr]: 
-  "hnr (master_assn' {(xs, xsi)}) (\<hole> :: ?'a Heap) ?\<Gamma>' (return_tuple_4 xs)"
+  "hnr (master_assn' (insert (xs, xsi) F)) (\<hole> :: ?'a Heap) ?\<Gamma>' (return_tuple_4 xs)"
   unfolding return_tuple_4_def
   by hnr_diff_arr
 
 synth_definition not_linear_diff_arr is [hnr_rule_diff_arr]:
-  "hnr (master_assn' {(xs, xsi)}) (\<hole> :: ?'a Heap) ?\<Gamma>' (not_linear xs)"
+  "hnr (master_assn' (insert (xs, xsi) F)) (\<hole> :: ?'a Heap) ?\<Gamma>' (not_linear xs)"
   unfolding not_linear_def 
   by hnr_diff_arr
 
 synth_definition if_1_diff_arr is [hnr_rule_diff_arr]:
-  "hnr (master_assn' {(xs, xsi)}) (\<hole> :: ?'a Heap) ?\<Gamma>' (if_1 xs)"
+  "hnr (master_assn' (insert (xs, xsi) F)) (\<hole> :: ?'a Heap) ?\<Gamma>' (if_1 xs)"
   unfolding if_1_def 
   by hnr_diff_arr
 
 synth_definition if_2_diff_arr is [hnr_rule_diff_arr]:
-  "hnr (master_assn' {(xs, xsi)}) (\<hole> :: ?'a Heap) ?\<Gamma>' (if_2 xs)"
+  "hnr (master_assn' (insert (xs, xsi) F)) (\<hole> :: ?'a Heap) ?\<Gamma>' (if_2 xs)"
   unfolding if_2_def 
   by hnr_diff_arr
 
 synth_definition if_3_diff_arr is [hnr_rule_diff_arr]:
-  "hnr (master_assn' {(xs, xsi)}) (\<hole> :: ?'a Heap) ?\<Gamma>' (if_3 xs)"
+  "hnr (master_assn' (insert (xs, xsi) F)) (\<hole> :: ?'a Heap) ?\<Gamma>' (if_3 xs)"
   unfolding if_3_def 
   by hnr_diff_arr
 
 synth_definition if_4_diff_arr is [hnr_rule_diff_arr]:
-  "hnr (master_assn' {(xs, xsi)}) (\<hole> :: ?'a Heap) ?\<Gamma>' (if_4 xs)"
+  "hnr (master_assn' (insert (xs, xsi) F)) (\<hole> :: ?'a Heap) ?\<Gamma>' (if_4 xs)"
   unfolding if_4_def 
   by hnr_diff_arr
 
@@ -301,7 +313,7 @@ synth_definition if_5_diff_arr is [hnr_rule_diff_arr]:
   by hnr_diff_arr
 
 synth_definition if_6_diff_arr is [hnr_rule_diff_arr]:
-  "hnr (master_assn' {(xs, xsi)}) (\<hole> :: ?'a Heap) ?\<Gamma>' (if_6 xs)"
+  "hnr (master_assn' (insert (xs, xsi) F)) (\<hole> :: ?'a Heap) ?\<Gamma>' (if_6 xs)"
   unfolding if_6_def 
   by hnr_diff_arr
 
@@ -311,12 +323,12 @@ synth_definition if_7_diff_arr is [hnr_rule_diff_arr]:
   by hnr_diff_arr
 
 synth_definition tuple_list_diff_arr is [hnr_rule_diff_arr]:
-  "hnr (master_assn' {(xs, xsi)}) (\<hole> :: ?'a Heap) ?\<Gamma>' (tuple_list xs)"
+  "hnr (master_assn' (insert (xs, xsi) F)) (\<hole> :: ?'a Heap) ?\<Gamma>' (tuple_list xs)"
   unfolding tuple_list_def 
   by hnr_diff_arr
 
 synth_definition nested_diff_arr is 
-  "hnr (master_assn' {(xs, xsi)}) (\<hole> :: ?'a Heap) ?\<Gamma>' (nested xs)"
+  "hnr (master_assn' (insert (xs, xsi) F)) (\<hole> :: ?'a Heap) ?\<Gamma>' (nested xs)"
   unfolding nested_def 
   by hnr_diff_arr
 
@@ -325,33 +337,45 @@ schematic_goal "hnr (master_assn' {(xs, xsi)}) (?c :: ?'a Heap) ?\<Gamma>' (fall
   unfolding fallback_1_def 
   by hnr_diff_arr
 
-schematic_goal "hnr emp (?c :: ?'a Heap) ?\<Gamma>' (create_list x)"
+synth_definition create_list_diff_arr is [hnr_rule_diff_arr]: 
+  "hnr emp (\<hole> :: ?'a Heap) ?\<Gamma>' (create_list x)"
   unfolding create_list_def 
   by hnr_diff_arr
 
-schematic_goal "hnr emp (?c :: ?'a Heap) ?\<Gamma>' (create_diff_arr_empty)"
+synth_definition create_diff_arr_empty_impl is [hnr_rule_diff_arr]: 
+  "hnr emp (\<hole> :: ?'a Heap) ?\<Gamma>' (create_diff_arr_empty)"
   unfolding create_diff_arr_empty_def 
   by hnr_diff_arr
 
-schematic_goal "hnr emp (?c :: ?'a Heap) ?\<Gamma>' (create_diff_arr x)"
+synth_definition create_diff_arr_impl is [hnr_rule_diff_arr]: 
+  "hnr emp (\<hole> :: ?'a Heap) ?\<Gamma>' (create_diff_arr x)"
   unfolding create_diff_arr_def 
   by hnr_diff_arr
 
 (* TODO: Nested lists *)
-schematic_goal "hnr emp (?c :: ?'a Heap) ?\<Gamma>' (create_diff_arr_2 x)"
+synth_definition create_diff_arr_2_impl is [hnr_rule_diff_arr]: 
+  "hnr emp (\<hole> :: ?'a Heap) ?\<Gamma>' (create_diff_arr_2 x)"
   unfolding create_diff_arr_2_def 
-  by hnr_diff_arr
+  apply hnr_step_diff_arr+
+  oops
                                                  
-schematic_goal "hnr emp (?c :: ?'a Heap) ?\<Gamma>' (create_diff_arr_3)"
+synth_definition create_diff_arr_3_impl is [hnr_rule_diff_arr]: 
+  "hnr emp (\<hole> :: ?'a Heap) ?\<Gamma>' (create_diff_arr_3)"
   unfolding create_diff_arr_3_def 
   by hnr_diff_arr
 
+synth_definition create_diff_arr_4_impl is [hnr_rule_diff_arr]: 
+  "hnr emp (\<hole> :: ?'a Heap) ?\<Gamma>' (create_diff_arr_4 x y)"
+  unfolding create_diff_arr_4_def 
+  by hnr_diff_arr
+
 (* TODO: Do I need a combined operator? *)
-schematic_goal "hnr emp (?c :: ?'a Heap) ?\<Gamma>' (create_arr_diff_arr x)"
+synth_definition create_diff_arr_arr_impl is [hnr_rule_diff_arr]: 
+  "hnr emp (\<hole> :: ?'a Heap) ?\<Gamma>' (create_arr_diff_arr x)"
   unfolding create_arr_diff_arr_def 
   apply hnr_arr
   by hnr_diff_arr
 
-export_code array_nth_safe array_update_safe in SML_imp
+export_code create_diff_arr_4_impl in SML_imp module_name foo
 
 end
